coq/examples/gemm_gemm_naive_gen.v
@@ -8,9 +8,20 @@ Module MS := MIRSemantics.
 Module Gemm_gemm_naive_gen.
 
 Definition prog : list M.stmt :=
-  [ M.SIf (M.EVar "_33") [ M.SIf (M.EVar "_34") [ M.SLoop [ M.SLoad "_44" (M.EVar "_1") M.TyF32;
-      M.SLoad "_51" (M.EVar "_2") M.TyF32 ];
+  [ M.SAssign "_17" (M.EVar "_18");
+    M.SAssign "_25" (M.EVar "_26");
+    M.SIf (M.EVar "_33") [ M.SIf (M.EVar "_34") [ M.SAssign "_35" (M.EVal (M.VF32 0));
+      M.SAssign "_38" (M.EVar "_36");
+      M.SLoop [ M.SLoad "_44" (M.EVar "_1") M.TyF32;
+      M.SLoad "_51" (M.EVar "_2") M.TyF32;
+      M.SAssign "_43" (M.EMul (M.EVar "_44") (M.EVar "_51"));
+      M.SAssign "_35" (M.EAdd (M.EVar "_35") (M.EVar "_43")) ];
+      M.SAssign "_68" (M.EVar "_59");
+      M.SAssign "_69" (M.EVar "_68");
+      M.SAssign "_65" (M.EVar "_35");
+      M.SAssign "_64" (M.EMul (M.EVar "_7") (M.EVar "_65"));
       M.SLoad "_67" (M.EVar "_58") M.TyF32;
+      M.SAssign "_66" (M.EMul (M.EVar "_8") (M.EVar "_67"));
       M.SStore (M.EVar "_58") (M.EAdd (M.EVar "_64") (M.EVar "_66")) M.TyU32 ] [] ] [] ].
 
 End Gemm_gemm_naive_gen.
