coq/examples/saxpy_gen.v
@@ -8,8 +8,13 @@ Module MS := MIRSemantics.
 Module Saxpy_gen.
 
 Definition prog : list M.stmt :=
-  [ M.SLoop [ M.SLoad "_10" (M.EPtrAdd (M.EVar "_2") (M.EVar "_8")) M.TyF32;
+  [ M.SAssign "_5" (M.EVal (M.VI32 0));
+    M.SAssign "_7" (M.EVar "_5");
+    M.SLoop [ M.SAssign "_9" (M.EVar "_5");
+      M.SAssign "_8" (M.EVar "_9");
+      M.SLoad "_10" (M.EPtrAdd (M.EVar "_2") (M.EVar "_8")) M.TyF32;
       M.SLoad "_12" (M.EPtrAdd (M.EVar "_3") (M.EVar "_8")) M.TyF32;
+      M.SAssign "_14" (M.EMul (M.EVar "_1") (M.EVar "_10"));
       M.SStore (M.EPtrAdd (M.EVar "_3") (M.EVar "_8")) (M.EAdd (M.EVar "_14") (M.EVar "_12")) M.TyF32 ] ].
 
 End Saxpy_gen.
