coq/examples/sha_sha256_incremental_gen.v
@@ -8,6 +8,11 @@ Module MS := MIRSemantics.
 Module Sha_sha256_incremental_gen.
 
 Definition prog : list M.stmt :=
-  [ M.SIf (M.EVar "_7") [] [] ].
+  [ M.SAssign "_7" (M.EVar "_8");
+    M.SIf (M.EVar "_7") [] [];
+    M.SAssign "_15" (M.EVar "_9");
+    M.SAssign "_21" (M.EVar "_3");
+    M.SAssign "_22" (M.EVar "_21");
+    M.SAssign "_18" (M.EVar "_16") ].
 
 End Sha_sha256_incremental_gen.
