coq/examples/sha_sha256_oneshot_gen.v
@@ -8,6 +8,10 @@ Module MS := MIRSemantics.
 Module Sha_sha256_oneshot_gen.
 
 Definition prog : list M.stmt :=
-  [ M.SIf (M.EVar "_5") [] [] ].
+  [ M.SAssign "_5" (M.EVar "_6");
+    M.SIf (M.EVar "_5") [] [];
+    M.SAssign "_13" (M.EVar "_2");
+    M.SAssign "_14" (M.EVar "_13");
+    M.SAssign "_10" (M.EVar "_8") ].
 
 End Sha_sha256_oneshot_gen.
